examples/l3-machine-code/m0/prog/m0_progScript.sml
@@ -101,4 +101,172 @@ val m0_TEMPORAL_PC_INTRO = Q.store_thm("m0_TEMPORAL_PC_INTRO",
 
 (* ------------------------------------------------------------------------ *)
 
+(*
+  Theorems for moving literal loads into the code pool (e.g. ldr r1, [pc, #4])
+*)
+
+val () = wordsLib.guess_lengths()
+
+val data_to_thumb2_def = Define`
+   data_to_thumb2 (w: word32) =
+   INR ((15 >< 8) w @@ (7 >< 0) w @@ (31 >< 24) w @@ (23 >< 16) w):
+   word16 + word32`
+
+val tm = data_to_thumb2_def |> SPEC_ALL |> concl |> rhs |> rand
+
+val byte_lem =
+   utilsLib.map_conv blastLib.BBLAST_PROVE
+      [``(31 >< 24) ^tm = (15 >< 8) w``,
+       ``(23 >< 16) ^tm = (7 >< 0) w``,
+       ``(15 >< 8) ^tm = (31 >< 24) w``,
+       ``(7 >< 0) ^tm = (23 >< 16) w``]
+
+val m0_instr_star = Q.prove(
+   `!a w.
+       {m0_instr (a, data_to_thumb2 w)} =
+       m0_MEM a ((7 >< 0) w) *
+       m0_MEM (a + 1w) ((15 >< 8) w) *
+       m0_MEM (a + 2w) ((23 >< 16) w) *
+       m0_MEM (a + 3w) ((31 >< 24) w)`,
+   srw_tac [wordsLib.WORD_ARITH_EQ_ss]
+       [pred_setTheory.INSERT_UNION_EQ, m0_instr_def, m0_MEM_def,
+        data_to_thumb2_def, set_sepTheory.STAR_def, set_sepTheory.SPLIT_def,
+        byte_lem]
+   \\ simp [boolTheory.FUN_EQ_THM]
+   \\ metis_tac []
+   )
+
+val m0_instr_star_not_disjoint = Q.prove(
+   `!a w p.
+      ~DISJOINT (m0_instr (a, data_to_thumb2 w)) p ==>
+        ({p} *
+         m0_MEM a ((7 >< 0) w) *
+         m0_MEM (a + 1w) ((15 >< 8) w) *
+         m0_MEM (a + 2w) ((23 >< 16) w) *
+         m0_MEM (a + 3w) ((31 >< 24) w) = SEP_F)`,
+   rw [set_sepTheory.STAR_def, set_sepTheory.SPLIT_def, m0_instr_def,
+       data_to_thumb2_def, m0_MEM_def, pred_setTheory.DISJOINT_DEF, byte_lem]
+   \\ simp [boolTheory.FUN_EQ_THM, set_sepTheory.SEP_F_def]
+   \\ Cases_on `(m0_c_MEM a,m0_d_word8 ((7 >< 0) w)) IN p`          \\ simp []
+   \\ Cases_on `(m0_c_MEM (a + 1w),m0_d_word8 ((15 >< 8) w)) IN p`  \\ simp []
+   \\ Cases_on `(m0_c_MEM (a + 2w),m0_d_word8 ((23 >< 16) w)) IN p` \\ simp []
+   \\ Cases_on `(m0_c_MEM (a + 3w),m0_d_word8 ((31 >< 24) w)) IN p` \\ simp []
+   \\ fs [pred_setTheory.INSERT_INTER]
+   )
+
+val MOVE_TO_TEMPORAL_M0_CODE_POOL = Q.store_thm
+  ("MOVE_TO_TEMPORAL_M0_CODE_POOL",
+   `!a w c p q.
+       TEMPORAL_NEXT M0_MODEL
+        (p *
+         m0_MEM a ((7 >< 0) w) *
+         m0_MEM (a + 1w) ((15 >< 8) w) *
+         m0_MEM (a + 2w) ((23 >< 16) w) *
+         m0_MEM (a + 3w) ((31 >< 24) w))
+        c
+        (q *
+         m0_MEM a ((7 >< 0) w) *
+         m0_MEM (a + 1w) ((15 >< 8) w) *
+         m0_MEM (a + 2w) ((23 >< 16) w) *
+         m0_MEM (a + 3w) ((31 >< 24) w)) =
+       TEMPORAL_NEXT M0_MODEL
+        (cond (DISJOINT (m0_instr (a, data_to_thumb2 w))
+              (BIGUNION (IMAGE m0_instr c))) * p)
+        ((a, data_to_thumb2 w) INSERT c)
+        q`,
+    REPEAT strip_tac
+    \\ once_rewrite_tac [GSYM temporal_stateTheory.TEMPORAL_NEXT_CODE]
+    \\ rewrite_tac [M0_MODEL_def, stateTheory.CODE_POOL,
+                    pred_setTheory.IMAGE_INSERT,
+                    pred_setTheory.IMAGE_EMPTY,
+                    pred_setTheory.BIGUNION_INSERT,
+                    pred_setTheory.BIGUNION_EMPTY]
+    \\ Cases_on `DISJOINT (m0_instr (a, data_to_thumb2 w))
+                          (BIGUNION (IMAGE m0_instr c))`
+    \\ rw [stateTheory.UNION_STAR, m0_instr_star, set_sepTheory.SEP_CLAUSES,
+           temporal_stateTheory.TEMPORAL_NEXT_FALSE_PRE,
+           AC set_sepTheory.STAR_ASSOC set_sepTheory.STAR_COMM]
+    \\ imp_res_tac m0_instr_star_not_disjoint
+    \\ fs [set_sepTheory.SEP_CLAUSES,
+           temporal_stateTheory.TEMPORAL_NEXT_FALSE_PRE,
+           AC set_sepTheory.STAR_ASSOC set_sepTheory.STAR_COMM]
+    )
+
+val MOVE_TO_M0_CODE_POOL = Q.store_thm("MOVE_TO_M0_CODE_POOL",
+   `!a w c p q.
+       SPEC M0_MODEL
+        (p *
+         m0_MEM a ((7 >< 0) w) *
+         m0_MEM (a + 1w) ((15 >< 8) w) *
+         m0_MEM (a + 2w) ((23 >< 16) w) *
+         m0_MEM (a + 3w) ((31 >< 24) w))
+        c
+        (q *
+         m0_MEM a ((7 >< 0) w) *
+         m0_MEM (a + 1w) ((15 >< 8) w) *
+         m0_MEM (a + 2w) ((23 >< 16) w) *
+         m0_MEM (a + 3w) ((31 >< 24) w)) =
+       SPEC M0_MODEL
+        (cond (DISJOINT (m0_instr (a, data_to_thumb2 w))
+                        (BIGUNION (IMAGE m0_instr c))) * p)
+        ((a, data_to_thumb2 w) INSERT c)
+        q`,
+    REPEAT strip_tac
+    \\ once_rewrite_tac [GSYM progTheory.SPEC_CODE]
+    \\ rewrite_tac [M0_MODEL_def, stateTheory.CODE_POOL,
+                    pred_setTheory.IMAGE_INSERT,
+                    pred_setTheory.IMAGE_EMPTY,
+                    pred_setTheory.BIGUNION_INSERT,
+                    pred_setTheory.BIGUNION_EMPTY]
+    \\ Cases_on `DISJOINT (m0_instr (a, data_to_thumb2 w))
+                          (BIGUNION (IMAGE m0_instr c))`
+    \\ rw [stateTheory.UNION_STAR, m0_instr_star, set_sepTheory.SEP_CLAUSES,
+           progTheory.SPEC_FALSE_PRE,
+           AC set_sepTheory.STAR_ASSOC set_sepTheory.STAR_COMM]
+    \\ imp_res_tac m0_instr_star_not_disjoint
+    \\ fs [set_sepTheory.SEP_CLAUSES, progTheory.SPEC_FALSE_PRE,
+           AC set_sepTheory.STAR_ASSOC set_sepTheory.STAR_COMM]
+    )
+
+val sub_intro = Theory.save_thm("sub_intro",
+   simpLib.SIMP_PROVE (srw_ss()) []
+      ``(a + (-b + c) = a - b + c : word32) /\ (a + -b = a - b)``
+   )
+
+val tac = asm_simp_tac (srw_ss()++wordsLib.WORD_CANCEL_ss)
+             [pred_setTheory.INSERT_INTER]
+
+(*
+val top = utilsLib.rhsc (wordsLib.WORD_EVAL_CONV ``word_T : word32``)
+*)
+
+val DISJOINT_m0_instr = Q.store_thm("DISJOINT_m0_instr",
+   `!a pc x y.
+      3w <+ a /\ a <+ 0xFFFFFFFDw ==>
+      DISJOINT (m0_instr (pc + a, data_to_thumb2 x)) (m0_instr (pc, INL y))`,
+   rw [m0_instr_def, data_to_thumb2_def, byte_lem, pred_setTheory.DISJOINT_DEF]
+   \\ `a + 1w <> 0w` by blastLib.FULL_BBLAST_TAC
+   \\ `a + 2w <> 0w` by blastLib.FULL_BBLAST_TAC
+   \\ `a + 3w <> 0w` by blastLib.FULL_BBLAST_TAC
+   \\ `a <> 0w` by blastLib.FULL_BBLAST_TAC
+   \\ `3w <> a` by blastLib.FULL_BBLAST_TAC
+   \\ `2w <> a` by blastLib.FULL_BBLAST_TAC
+   \\ `1w <> a` by blastLib.FULL_BBLAST_TAC
+   \\ tac
+   )
+
+fun disjoint_m0_instr q =
+   DISJOINT_m0_instr
+   |> Q.SPEC q
+   |> Drule.SPEC_ALL
+   |> Conv.CONV_RULE (LAND_CONV blastLib.BBLAST_CONV)
+   |> REWRITE_RULE []
+   |> Drule.GEN_ALL
+
+val disjoint_m0_instr_thms = Theory.save_thm("disjoint_m0_instr_thms",
+   disjoint_m0_instr `w2w (w: word10) + 4w`
+   )
+
+(* ------------------------------------------------------------------------ *)
+
 val () = export_theory()
